removing a bunch of comments/dead code

theories/Lambda/ExprSubst.v
@@ -14,6 +14,8 @@ Require Import MirrorCore.EnvI.
 Require Import MirrorCore.SymI.
 Require Import MirrorCore.ExprI.
 Require Import MirrorCore.TypesI.
+Require Import MirrorCore.InstantiateI.
+Require Import MirrorCore.Util.Forwardy.
 Require Import MirrorCore.Lambda.ExprCore.
 Require Import MirrorCore.Lambda.ExprD.
 Require Import MirrorCore.Lambda.ExprLift.
@@ -27,21 +29,8 @@ Section mentionsU.
   Variable typ : Type.
   Variable func : Type.
 
-  Section param.
-    Variable u : uvar.
-
-    Fixpoint mentionsU (e : expr typ func) : bool :=
-      match e with
-        | Var _
-        | Inj _ => false
-        | UVar u' => EqNat.beq_nat u u'
-        | App f e => if mentionsU f then true else mentionsU e
-        | Abs _ e => mentionsU e
-      end.
-  End param.
-
   Lemma mentionsU_lift : forall u e a b,
-    mentionsU u (lift a b e) = mentionsU u e.
+    mentionsU u (lift (typ := typ) (func := func) a b e) = mentionsU u e.
   Proof.
     induction e; simpl; intros; intuition;
     Cases.rewrite_all_goal; intuition.
@@ -95,11 +84,11 @@ Section instantiate.
 
 End instantiate.
 
-Section strengthen.
-  Context {typ : Type}.
-  Context {func : Type}.
-  Context {RType_typD : RType typ}.
-  Context {Typ2_Fun : Typ2 RType_typD Fun}.
+Section instantiate_thm.
+  Variable typ : Type.
+  Variable func : Type.
+  Variable RType_typ : RType typ.
+  Variable Typ2_Fun : Typ2 _ Fun.
   Context {RSym_func : RSym func}.
 
   (** Reasoning principles **)
@@ -107,711 +96,208 @@ Section strengthen.
   Context {Typ2Ok_Fun : Typ2Ok Typ2_Fun}.
   Context {RSymOk_func : RSymOk RSym_func}.
 
-  Lemma typeof_expr_strengthen
-  : forall ts tus tu (e : expr typ func) tvs (t : typ),
-      mentionsU (length tus) e = false ->
-      typeof_expr ts (tus ++ tu :: nil) tvs e = Some t ->
-      typeof_expr ts tus tvs e = Some t.
-  Proof.
-    induction e; simpl; intros; forward; inv_all; subst; auto.
-    { erewrite H3; eauto.
-      erewrite IHe2; eauto. }
-    { erewrite IHe; eauto. }
-    { rewrite nth_error_app_L in H0; auto.
-      eapply nth_error_length_lt in H0.
-      rewrite app_length in H0.
-      simpl in *.
-      consider (EqNat.beq_nat (length tus) u); try congruence.
-      intros. omega. }
-  Qed.
+  Let Expr_expr := @Expr_expr _ _ RType_typ _ _.
 
-  Lemma exprD'_strengthen
-  : forall ts tus tu (e : expr typ func) tvs (t : typ) eD,
-      mentionsU (length tus) e = false ->
-      exprD' ts (tus ++ tu :: nil) tvs t e = Some eD ->
-      exists eD',
-        exprD' ts tus tvs t e = Some eD' /\
-        forall us u vs,
-          eD (hlist_app us (Hcons u Hnil)) vs = eD' us vs.
-  Proof.
-    induction e; simpl; intros;
-    autorewrite with exprD_rw in *; simpl in *; forward; inv_all; subst; eauto.
-    { erewrite typeof_expr_strengthen by eauto.
-      eapply IHe2 in H5; eauto.
-      eapply H4 in H1; eauto.
-      forward_reason.
-      Cases.rewrite_all_goal.
-      eexists; split; eauto. intros.
-      unfold Open_App. simpl.
-      unfold OpenT, ResType.OpenT.
-      repeat first [ rewrite eq_Const_eq | rewrite eq_Arr_eq ].
-      rewrite H5. rewrite H6. reflexivity. }
-    { destruct (typ2_match_case ts t0) as [ [ ? [ ? [ ? ? ] ] ] | ? ].
-      { rewrite H1 in *.
-        unfold Relim in *.
-        red in x1. subst.
-        repeat first [ rewrite eq_Const_eq in *
-                     | rewrite eq_option_eq in *
-                     | rewrite eq_Arr_eq  in * ].
-        forward. inv_all; subst.
-        eapply IHe in H3; eauto.
-        forward_reason. rewrite H2. eexists; split; eauto.
-        intros. unfold OpenT, ResType.OpenT.
-        repeat first [ rewrite eq_Const_eq | rewrite eq_Arr_eq ].
-        clear - H3.
-        destruct (eq_sym (typ2_cast ts x x0)).
-        eapply functional_extensionality.
-        eauto. }
-      { rewrite H1 in *. congruence. } }
-    { cut (u < length tus).
-      { intro.
-        eapply nth_error_get_hlist_nth_appL with (tvs' := tu :: nil) (F := typD ts) in H0.
-        rewrite H1 in H0.
-        forward_reason. inv_all; subst. simpl in *.
-        rewrite H3. rewrite H2. eexists; split; eauto.
-        simpl. intros. rewrite H4. eauto. }
-      { eapply nth_error_get_hlist_nth_Some in H1.
-        destruct H1. clear H0. simpl in *.
-        eapply nth_error_length_lt in x0.
-        rewrite app_length in x0.
-        consider (EqNat.beq_nat (length tus) u); try congruence.
-        intros. simpl in *. omega. } }
-  Qed.
-End strengthen.
-
-(*
-  Theorem typeof_expr_instantiate : forall tu tg,
-    (forall u e',
-       lookup u = Some e' ->
-       exists t',
-         nth_error tu u = Some t' /\
-         typeof_expr tu tg e' = Some t') ->
-    forall e tg',
-      typeof_expr tu (tg' ++ tg) (instantiate (length tg') e) =
-      typeof_expr tu (tg' ++ tg) e.
-  Proof.
-    induction e; simpl; intros;
-    repeat match goal with
-             | H : _ |- _ =>
-               rewrite H
-           end; auto.
-    { specialize (IHe (t :: tg')). simpl in *.
-      rewrite IHe. reflexivity. }
-    { consider (lookup u); intros; simpl; auto.
-      specialize (H _ _ H0). destruct H.
-      intuition.
-      generalize (typeof_expr_lift _ tu nil tg' tg e); simpl.
-      congruence. }
-  Qed.
-
-  Theorem exprD'_instantiate : forall us gs',
-    (forall u e',
-       lookup u = Some e' ->
-       exists tval,
-         nth_error us u = Some tval /\
-         exprD us gs' e' (projT1 tval) = Some (projT2 tval)) ->
-    forall e t v,
-      let (tv',vs') := EnvI.split_env gs' in
-      let (tu',us') := EnvI.split_env us in
-      match ExprD.exprD' tu' (v ++ tv') e t,
-            ExprD.exprD' tu' (v ++ tv') (instantiate (length v) e) t
-      with
-        | Some l , Some r => forall vs,
-                               l us' (hlist_app vs vs') = r us' (hlist_app vs vs')
-        | None , None => True
-        | _ , _ => False
-      end.
-  Proof.
-    unfold exprD. intros us gs'.
-    consider (split_env us). intros x h Hsplit_env.
-    destruct (split_env gs'). intros Hlookup.
-    Opaque exprD'.
-    induction e; simpl; intros; autorewrite with exprD_rw; auto.
-    { forward. }
-    { forward. }
-    { rewrite typeof_expr_instantiate.
-      { consider (typeof_expr x (v ++ x0) e1); auto.
-        destruct t0; auto.
-        specialize (IHe1 (tyArr t0_1 t0_2) v).
-        specialize (IHe2 t0_1 v).
-        repeat match goal with
-                 | _ : context [ match ?X with _ => _ end ] |- _ =>
-                   consider X; try congruence; intros
-                 | |- context [ match ?X with _ => _ end ] =>
-                   consider X; try congruence; intros
-               end; auto.
-        inv_all; subst. rewrite IHe2. rewrite IHe1. reflexivity. }
-      { clear - Hlookup Hsplit_env.
-        intros. specialize (Hlookup _ _ H).
-        destruct Hlookup. intuition.
-        unfold ExprI.exprD' in H2. simpl in H2.
-        forward; inv_all; subst.
-        exists (projT1 x1).
-        apply split_env_nth_error in H1.
-        rewrite Hsplit_env in *. simpl in *.
-        generalize dependent (hlist_nth h u).
-        forward. subst; simpl.
-        split; eauto. simpl in *.
-        consider (ExprD.exprD' x x0 e' t0); try congruence; intros.
-        eapply ExprD.typeof_expr_exprD'. eauto. } }
-    { destruct t0; auto.
-      specialize (IHe t0_2 (t :: v)). simpl in *.
-      repeat match goal with
-                 | _ : context [ match ?X with _ => _ end ] |- _ =>
-                   consider X; try congruence; intros
-                 | |- context [ match ?X with _ => _ end ] =>
-                   consider X; try congruence; intros
-               end; inv_all; subst; auto.
-      eapply functional_extensionality. intros.
-      specialize (IHe (Hcons x1 vs)). simpl in *; auto. }
-    { specialize (Hlookup u).
-      destruct (lookup u).
-      { specialize (Hlookup _ eq_refl).
-        forward_reason.
-        forward. inv_all; subst.
-        rewrite exprD'_type_cast.
-        generalize (exprD'_lift _ x nil v x0 e (projT1 x1)).
-        simpl. simpl in H0. rewrite H0.
-        forward.
-        erewrite ExprD3.EXPR_DENOTE_core.exprD'_typeof by eauto.
-        rewrite H2.
-        match goal with
-          | |- match match ?X with _ => _ end with _ => _ end =>
-            consider X; intros; forward
-        end.
-        { eapply EnvI.nth_error_get_hlist_nth_Some in H5.
-          forward_reason. simpl in *. subst.
-          apply split_env_nth_error in H.
-          rewrite Hsplit_env in *. simpl in *.
-          specialize (H5 h).
-          match goal with
-            | H : _ = match _ with eq_refl => ?X end , H' : _ ?Y |- _ =>
-              change X with Y in H ; generalize dependent Y
-          end.
-          rewrite x3. intros; subst; simpl in *.
-          match goal with
-            | |- match match ?x with _ => _ end with Some _ => match match ?y with _ => _ end with _ => _ end | _ => _ end =>
-              change y with x ; consider x
-          end; auto.
-          intros.
-          f_equal. specialize (H3 h Hnil). simpl in *.
-          rewrite H3. auto. }
-        { inv_all; subst.
-          eapply EnvI.nth_error_get_hlist_nth_None in H4.
-          clear - H H4 Hsplit_env.
-          apply split_env_nth_error in H.
-          rewrite Hsplit_env in *. simpl in *.
-          generalize dependent (hlist_nth h u).
-          rewrite H4. auto. } }
-      { clear Hlookup.
-        autorewrite with exprD_rw.
-        forward. } }
-  Qed.
-
-  Lemma typeof_expr_instantiate_Some
-  : forall (*lookup : uvar -> option (expr func)*) (tu : list typ)
-           (tg : tenv typ),
-      (forall (u : uvar) (e' : expr func) t',
-         lookup u = Some e' ->
-         nth_error tu u = Some t' ->
-         typeof_expr tu tg e' = Some t') ->
-      forall (e : expr func) (tg' : list typ) t,
-        typeof_expr tu (tg' ++ tg) e = Some t ->
-        typeof_expr tu (tg' ++ tg) (instantiate (length tg') e) = Some t.
-  Proof.
-    clear. induction e; simpl; intros; auto; forward.
-    { eapply IHe1 in H0. eapply IHe2 in H1.
-      Cases.rewrite_all_goal. reflexivity. }
-    { inv_all; subst.
-      eapply (IHe (t :: tg')) in H0.
-      simpl in H0. rewrite H0. reflexivity. }
-    { eapply H in H1; eauto.
-      generalize (@typeof_expr_lift _ _ RSym_func tu nil tg' tg e).
-      simpl. congruence. }
-  Qed.
-
-  Lemma exprD'_instantiate_Some
-  : forall tus tvs P,
-      (forall u t' e get,
-         nth_error_get_hlist_nth _ tus u = Some (@existT _ _ t' get) ->
-         lookup u = Some e ->
-         exists eD,
-           exprD' tus tvs e t' = Some eD /\
-           forall us vs,
-             P us vs ->
-             eD us vs = get us) ->
-      forall e tvs' t eD,
-        exprD' tus (tvs' ++ tvs) e t = Some eD ->
-        exists eD',
-          exprD' tus (tvs' ++ tvs) (instantiate (length tvs') e) t = Some eD' /\
-          forall us vs' vs,
-            P us vs ->
-            eD us (hlist_app vs' vs) = eD' us (hlist_app vs' vs).
-  Proof.
-    clear.
-    induction e; simpl; intros; eauto.
-    { red_exprD.
-      forward; inv_all; subst.
-      specialize (IHe1 _ _ _ H2); clear H2.
-      specialize (IHe2 _ _ _ H3); clear H3.
-      eapply typeof_expr_instantiate_Some in H1; eauto.
-      { forward_reason.
-        Cases.rewrite_all_goal.
-        rewrite typ_cast_typ_refl. eexists; split; eauto.
-        simpl. intros.
-        rewrite H4; eauto.
-        rewrite H3; eauto. }
-      { clear - H.
-        intros.
-        specialize (H u t' e').
-        consider (nth_error_get_hlist_nth (typD ts nil) tus u); intros.
-        { destruct s.
-          generalize H.
-          eapply nth_error_get_hlist_nth_Some in H. simpl in *.
-          forward_reason.
-          rewrite x0 in H1. inv_all; subst.
-          intros.
-          specialize (H2 _ H1 H0). destruct H2 as [ ? [ ? ? ] ].
-          clear H H1.
-          rewrite exprD'_type_cast in H2.
-          forward. inv_all; subst. reflexivity. }
-        { exfalso. eapply nth_error_get_hlist_nth_None in H.
-          congruence. } } }
-    { red_exprD.
-      forward; inv_all; subst.
-      specialize (IHe (t :: tvs') t2 _ H2).
-      simpl in IHe.
-      forward_reason.
-      rewrite H0.
-      eexists; split; eauto.
-      simpl. intros.
-      eapply functional_extensionality. intros.
-      exact (H1 us (Hcons x0 vs') vs X). }
-    { consider (lookup u); intros.
-      { red_exprD.
-        forward; inv_all; subst.
-        specialize (H _ _ _ _ H2 H1).
-        forward_reason.
-        generalize (@exprD'_lift _ _ RSym_func tus nil tvs' tvs e t).
-        simpl. rewrite H.
-        intros. forward.
-        eexists; split; eauto.
-        intros.
-        erewrite <- H0. symmetry. eapply (H4 us Hnil vs' vs). apply X. }
-      { eauto. } }
-  Qed.
-
-End instantiate.
-*)
-
-(*
-
-  Theorem mentionsU_substU : forall u u' e' e under,
-    mentionsU u (substU u' e under e') =
-    if u ?[ eq ] u' then
-      if mentionsU u e' then mentionsU u e else false
-    else
-      if mentionsU u e' then true else if mentionsU u' e' then mentionsU u e else false.
-  Proof.
-    induction e'; simpl; try congruence; intros;
-    repeat match goal with
-             | H : _ |- _ =>
-               match type of H with
-                 | not (eq _ _) => fail 1
-                 | _ -> False => fail 1
-                 | ?T => rewrite H by eauto
-               end
-             | |- context [ if @rel_dec ?A ?B ?C ?X ?Y then _ else _ ] =>
-               consider (@rel_dec A B C X Y); try congruence; intros; auto; subst
-             | |- context [ if EqNat.beq_nat ?X ?Y then _ else _ ] =>
-               consider (EqNat.beq_nat X Y); try congruence; intros; subst; auto; subst
-             | |- _ =>
-               progress ( rewrite mentionsU_lift in * )
-             | |- context [ if mentionsU ?X ?Y then _ else _ ] =>
-               consider (mentionsU X Y); try congruence; intros; subst; auto
-           end; simpl in *; eauto.
-    consider (EqNat.beq_nat u' u0); congruence.
-    consider (EqNat.beq_nat u0 u0); congruence.
-    consider (EqNat.beq_nat u u0); congruence.
-  Qed.
-
-  Lemma mentionsU_WellTyped : forall tu e tv t,
-    WellTyped_expr tu tv e t ->
-    forall n : uvar, length tu <= n -> mentionsU n e = false.
+  Lemma typeof_expr_instantiate
+  : forall f tus tvs,
+      (forall u e, f u = Some e ->
+                   typeof_expr nil tus tvs e = nth_error tus u) ->
+      forall e tvs',
+        typeof_expr nil tus (tvs' ++ tvs) e =
+        typeof_expr nil tus (tvs' ++ tvs) (instantiate f (length tvs') e).
   Proof.
     induction e; simpl; intros; auto.
-    { rewrite WellTyped_expr_App in H.
-      do 2 destruct H. intuition.
-      erewrite IHe1; eauto. }
-    { rewrite WellTyped_expr_Abs in H.
-      destruct H; intuition; subst.
-      eapply IHe; eauto. }
-    { rewrite WellTyped_expr_UVar in *.
-      consider (EqNat.beq_nat n u); intros; auto.
-      subst. exfalso.
-      rewrite <- (app_nil_r tu) in H.
-      rewrite nth_error_app_R in *; auto.
-      destruct (u - length tu); inversion H. }
+    { rewrite (IHe1 tvs').
+      rewrite (IHe2 tvs').
+      reflexivity. }
+    { specialize (IHe (t :: tvs')).
+      simpl in IHe.
+      rewrite IHe. reflexivity. }
+    { specialize (H u).
+      destruct (f u).
+      { specialize (typeof_expr_lift nil tus e nil tvs' tvs).
+        simpl.
+        intro XXX; change_rewrite XXX; clear XXX.
+        symmetry. eapply H; reflexivity. }
+      { reflexivity. } }
   Qed.
 
-  Theorem typeof_expr_mentionsU_strengthen : forall tu e tg t',
-    mentionsU (length tu) e = false ->
-    typeof_expr (tu ++ t' :: nil) tg e =
-    typeof_expr tu tg e.
+  Lemma typeof_expr_instantiate'
+  : forall f tus tvs,
+      (forall u e t, f u = Some e ->
+                     nth_error tus u = Some t ->
+                     typeof_expr nil tus tvs e = Some t) ->
+      forall e tvs' t,
+        typeof_expr nil tus (tvs' ++ tvs) e = Some t ->
+        typeof_expr nil tus (tvs' ++ tvs) (instantiate f (length tvs') e) = Some t.
   Proof.
-    induction e; simpl; intros;
-    repeat match goal with
-             | _ : context [ match ?X with _ => _ end ] |- _ =>
-               consider X; intros; try congruence
-             | H : _ |- _ =>
-               erewrite H by eauto
-           end; auto.
-    destruct (Compare_dec.lt_eq_lt_dec (length tu) u) as [ [ | ] | ].
-    { rewrite nth_error_past_end.
-      rewrite nth_error_past_end; auto.
-      omega. rewrite app_length. simpl. omega. }
-    { consider (EqNat.beq_nat (length tu) u); try congruence. }
-    { rewrite nth_error_app_L by auto. auto. }
+    induction e; simpl; intros; auto.
+    { forwardy.
+      erewrite IHe1 by eassumption.
+      erewrite IHe2 by eassumption.
+      eassumption. }
+    { specialize (IHe (t :: tvs')).
+      simpl in IHe.
+      forwardy.
+      erewrite IHe by eassumption. eassumption. }
+    { specialize (H u).
+      destruct (f u).
+      { specialize (typeof_expr_lift nil tus e nil tvs' tvs).
+        simpl.
+        intro XXX; change_rewrite XXX; clear XXX.
+        eapply H; eauto. }
+      { eapply H0. } }
   Qed.
 
-  Lemma typeof_expr_mentionsU_strengthen_multi_lem : forall tu tu' e tg,
-    (forall n, length tu <= n -> mentionsU n e = false) ->
-    typeof_expr (tu ++ rev tu') tg e =
-    typeof_expr tu tg e.
+  Theorem exprD'_instantiate
+  : @exprD'_instantiate typ (expr typ func) RType_typ Expr_expr (@instantiate typ func).
   Proof.
-    intros. induction tu'; simpl.
-    { rewrite app_nil_r. reflexivity. }
-    { rewrite <- app_ass.
-      rewrite typeof_expr_mentionsU_strengthen.
-      eapply IHtu'.
-      rewrite app_length. rewrite H; auto.
-      omega. }
+    red. induction e; simpl; intros; eauto.
+    { autorewrite with exprD_rw in *; eauto.
+      simpl in *.
+      forwardy.
+      eapply typeof_expr_instantiate' with (f := f) in H0.
+      change_rewrite H0.
+      specialize (IHe1 tvs' (typ2 y t) _ _ H H1).
+      specialize (IHe2 _ _ _ _ H H2).
+      forward_reason.
+      change_rewrite H5. change_rewrite H4.
+      eexists; split; [ reflexivity | ].
+      intros. inv_all; subst.
+      unfold Open_App, OpenT, ResType.OpenT.
+      autorewrite with eq_rw.
+      rewrite H6 by assumption.
+      rewrite H7 by assumption. reflexivity.
+      clear - H RTypeOk_typD Typ2Ok_Fun RSymOk_func.
+      red in H.
+      intros.
+      specialize (fun t get => H u e t get H0).
+      simpl in *.
+      consider (nth_error_get_hlist_nth (typD nil) tus u).
+      { intros. destruct s.
+        specialize (H2 _ _ H).
+        forward_reason.
+        eapply nth_error_get_hlist_nth_Some in H.
+        simpl in H. forward_reason.
+        rewrite x1 in H1. inv_all; subst.
+        eapply exprD'_typeof_expr; eauto. }
+      { intro. exfalso.
+        eapply nth_error_get_hlist_nth_None in H. congruence. } }
+    { autorewrite with exprD_rw in *.
+      destruct (typ2_match_case nil t0) as [ [ ? [ ? [ ? ? ] ] ] | ? ].
+      { rewrite H1 in *. clear H1.
+        simpl in *.
+        unfold Relim in *.
+        autorewrite with eq_rw in *.
+        forwardy.
+        Cases.rewrite_all_goal.
+        specialize (IHe (t :: tvs')_ _ _ H H3).
+        forward_reason.
+        simpl in *.
+        Cases.rewrite_all_goal.
+        eexists; split; eauto.
+        intros.
+        inv_all; subst.
+        unfold OpenT, ResType.OpenT.
+        autorewrite with eq_rw.
+        eapply match_eq_match_eq.
+        eapply match_eq_match_eq with (F := fun x => x).
+        apply functional_extensionality.
+        intro. eapply (H6 us vs (Hcons (Rcast_val y1 x3) vs')); auto. }
+      { rewrite H1 in H0.
+        exfalso. congruence. } }
+    { red in H.
+      specialize (H u).
+      destruct (f u).
+      { autorewrite with exprD_rw in *; simpl in *.
+        forwardy.
+        specialize (H _ _ _ eq_refl H0).
+        forward_reason.
+        generalize (exprD'_lift nil tus e nil tvs' tvs t).
+        destruct y.
+        simpl. change_rewrite H.
+        intros; forwardy.
+        eexists; split; [ eassumption | ].
+        intros.
+        inv_all; subst.
+        erewrite H3 by eauto. eapply (H5 us Hnil vs' vs). }
+      { clear H.
+        eexists; split; [ eassumption | ].
+        reflexivity. } }
   Qed.
 
-  Theorem typeof_expr_mentionsU_strengthen_multi : forall tu tu' e tg,
-    (forall n, length tu <= n -> mentionsU n e = false) ->
-    typeof_expr (tu ++ tu') tg e =
-    typeof_expr tu tg e.
+  Theorem if_true_iff
+  : forall T (a : bool) (b c d : T),
+      (if a then b else c) = d <->
+      ((a = true /\ b = d) /\ (a = false /\ c = d)).
   Proof.
-    intros.
-    rewrite <- (rev_involutive tu').
-    eapply typeof_expr_mentionsU_strengthen_multi_lem. auto.
-  Qed.
+  Admitted.
 
-  Lemma exprD'_mentionsU_strengthen : forall tu u e,
-    mentionsU (length tu) e = false ->
-    forall tg t,
-    match ExprD.exprD' (tu ++ u :: nil) tg e t
-        , ExprD.exprD' tu tg e t
-    with
-      | None , None => True
-      | Some l , Some r => forall us uv vs,
-                             l (hlist_app us (Hcons uv Hnil)) vs = r us vs
-      | _ , _ => False
-    end.
+  Theorem instantiate_mentionsU
+  : @instantiate_mentionsU typ (expr typ func) RType_typ Expr_expr (@instantiate typ func).
   Proof.
-    induction e; simpl; intros; autorewrite with exprD_rw;
-    repeat match goal with
-             | _ : context [ match ?X with _ => _ end ] |- _ =>
-               consider X; try congruence; intros
-           end.
-    { forward. }
-    { forward. }
-    { forward_reason.
-      repeat rewrite typeof_expr_mentionsU_strengthen by eauto.
-      forward. subst.
-      specialize (H0 tg (tyArr t1 t2)).
-      specialize (IHe2 tg t1).
-      repeat match goal with
-               | _ : context [ match ?X with _ => _ end ] |- _ =>
-                 consider X; try congruence; intros
-               | |- context [ match ?X with _ => _ end ] =>
-                 consider X; try congruence; intros
-             end; inv_all; subst; auto.
-      rewrite H4. rewrite IHe2. reflexivity. }
-    { destruct t0; auto.
-      specialize (IHe H (t :: tg) t0_2).
-      repeat match goal with
-               | _ : context [ match ?X with _ => _ end ] |- _ =>
-                 consider X; try congruence; intros
-               | |- context [ match ?X with _ => _ end ] =>
-                 consider X; try congruence; intros
-             end; inv_all; subst; auto.
-      eapply functional_extensionality; eauto. }
-    { destruct (Compare_dec.lt_eq_lt_dec (length tu) u0) as [ [ | ] | ].
-      { match goal with
-          | |- match match ?X with _ => _ end with _ => _ end =>
-            consider X; intros
-        end.
-        { eapply nth_error_get_hlist_nth_appR in H0; eauto with typeclass_instances.
-          2: omega.
-          simpl in *. forward_reason.
-          exfalso.
-          consider (u0 - length tu).
-          { intros. exfalso. omega. }
-          { congruence. } }
-        { forward. subst. inv_all; subst.
-          apply EnvI.nth_error_get_hlist_nth_Some in H2.
-          forward_reason. simpl in *.
-          clear - x l.
-          apply nth_error_length_lt in x. omega. } }
-      { exfalso.
-        consider (EqNat.beq_nat (length tu) u0); congruence. }
-      { generalize l.
-        eapply nth_error_get_hlist_nth_appL with (F := typD ts nil) (tvs' := u :: nil) in l; eauto with typeclass_instances.
-        forward_reason. simpl in *.
-        repeat match goal with
-          | H : ?X = _ |- context [ ?Y ] =>
-            change Y with X ; rewrite H
-        end.
-        forward. simpl in *. forward.
-        subst. f_equal. auto. } }
+    clear.
+    red. intros f n e u. revert n.
+    induction e; simpl; intros.
+    { split; intros. congruence.
+      destruct H. destruct H; auto.
+      forward_reason; auto. }
+    { split; intros. congruence.
+      destruct H. destruct H; auto.
+      forward_reason; auto. }
+    { specialize (IHe1 n). specialize (IHe2 n).
+      simpl in *.
+      transitivity (mentionsU u (instantiate f n e1) = true \/ mentionsU u (instantiate f n e2) = true).
+      { destruct (mentionsU u (instantiate f n e1)); intuition. }
+      { rewrite IHe1. rewrite IHe2.
+        split.
+        { destruct 1.
+          { destruct H; forward_reason.
+            { rewrite H0. left; auto. }
+            { right. do 2 eexists; split; [ eassumption | ].
+              rewrite H0. eauto. } }
+          { destruct H; forward_reason.
+            { rewrite H. rewrite H0.
+              left. split; auto. destruct (mentionsU u e1); reflexivity. }
+            { right. do 2 eexists; split; eauto.
+              split; auto.
+              destruct (mentionsU x e1); eauto. } } }
+        { destruct 1; forward_reason.
+          { rewrite H. destruct (mentionsU u e1).
+            { left. left; auto. }
+            { right; left; auto. } }
+          { consider (mentionsU x e1).
+            { left; right. do 2 eexists; split; eauto. }
+            { intros. right; right; do 2 eexists; split; eauto. } } } } }
+    { specialize (IHe (S n)). simpl in IHe. eapply IHe. }
+    { split.
+      { consider (EqNat.beq_nat u u0).
+        { intros; subst.
+          consider (f u0).
+          + intros. right.
+            rewrite mentionsU_lift in H0.
+            do 2 eexists; split; eauto.
+            split. consider (EqNat.beq_nat u0 u0); auto. auto.
+          + intros. left; auto. }
+        { intros. right.
+          consider (f u0); intros.
+          { do 2 eexists.
+            split; eauto. rewrite mentionsU_lift in H1.
+            split; auto.
+            consider (EqNat.beq_nat u0 u0); auto. }
+          { simpl in H1.
+            exfalso.
+            consider (EqNat.beq_nat u u0). apply H. } } }
+      { intros. destruct H.
+        { destruct H.
+          consider (EqNat.beq_nat u u0).
+          intros; subst.
+          rewrite H. simpl.
+          consider (EqNat.beq_nat u0 u0); auto. }
+        { forward_reason.
+          consider (EqNat.beq_nat x u0).
+          intros; subst.
+          rewrite H. rewrite mentionsU_lift. assumption. } } }
   Qed.
 
-  Lemma exprD'_mentionsU_strengthen_multi_lem : forall tu e,
-    (forall n, length tu <= n -> mentionsU n e = false) ->
-    forall tg t tu',
-      match ExprD.exprD' (tu ++ rev tu') tg e t
-          , ExprD.exprD' tu tg e t
-      with
-        | None , None => True
-        | Some l , Some r => forall us us' vs,
-                               l (hlist_app us us') vs = r us vs
-        | _ , _ => False
-      end.
-  Proof.
-    induction tu'; intros; simpl.
-    { consider (exprD' tu tg e t); intros.
-      { consider (exprD' (tu ++ nil) tg e t); intros.
-        { rewrite (hlist_eta us').
-          assert (tu ++ nil = tu) by (rewrite app_nil_r; auto).
-          clear - H0 H1 H2.
-          assert (hlist_app us Hnil = match eq_sym H2 in _ = t return hlist _ t with
-                                        | eq_refl => us
-                                      end).
-          { clear.
-            induction us. uip_all. reflexivity.
-            simpl in *.
-            uip_all.
-            inversion e. specialize (IHus (eq_sym H0)).
-            rewrite IHus. uip_all. clear.
-            revert us.
-            revert e. rewrite <- e0.
-            intros. uip_all. reflexivity. }
-          { rewrite H.
-            revert H0. revert H1. clear.
-            revert t1. revert t0. rewrite H2.
-            intros. rewrite H1 in *.
-            inv_all. subst t0.
-            simpl. reflexivity. } }
-        { assert (exprD' tu tg e t <> None) by congruence.
-          clear - H1 H2.
-          rewrite app_nil_r in H1. congruence. } }
-      { forward.
-        assert (exprD' (tu ++ nil) tg e t <> None) by congruence.
-        clear - H0 H2.
-        rewrite app_nil_r in H2. congruence. } }
-    { assert (mentionsU (length (tu ++ rev tu')) e = false).
-      { rewrite H; auto. rewrite app_length; omega. }
-      generalize (exprD'_mentionsU_strengthen (tu ++ rev tu') a e H0 tg t).
-      consider (exprD' (tu ++ rev tu') tg e t);
-        consider (exprD' tu tg e t); intros; auto; forward.
-      { consider (exprD' (tu ++ rev tu' ++ a :: nil) tg e t); intros.
-        { generalize (hlist_app_hlist_split _ _ us').
-          destruct (hlist_split (rev tu') (a :: nil) us').
-          simpl in *.
-          specialize (IHtu' us h vs).
-          specialize (H4 (hlist_app us h) (hlist_hd h0) vs).
-          intros. rewrite <- IHtu'. rewrite <- H4.
-          subst. rewrite hlist_app_assoc; eauto with typeclass_instances.
-          rewrite (hlist_eta h0). rewrite (hlist_eta (hlist_tl h0)).
-          simpl in *.
-          uip_all.
-          generalize (hlist_app us (hlist_app h (Hcons (hlist_hd h0) Hnil))).
-          generalize dependent t2; generalize dependent t3.
-          clear. revert e0.
-          rewrite <- (@app_ass typ). uip_all.
-          rewrite H3 in H5. inv_all; subst; auto. }
-        { clear - H3 H5.
-          generalize dependent t2.
-          rewrite app_ass. rewrite H5. congruence. } }
-      { rewrite app_ass in H4. congruence. } }
-  Qed.
-
-  Theorem exprD'_mentionsU_strengthen_multi : forall tu e,
-    (forall n, length tu <= n -> mentionsU n e = false) ->
-    forall tg t tu',
-      match ExprD.exprD' (tu ++ tu') tg e t
-          , ExprD.exprD' tu tg e t
-      with
-        | None , None => True
-        | Some l , Some r => forall us us' vs,
-                               l (hlist_app us us') vs = r us vs
-        | _ , _ => False
-      end.
-  Proof.
-    intros.
-    rewrite <- (rev_involutive tu').
-    eapply exprD'_mentionsU_strengthen_multi_lem. auto.
-  Qed.
-
-  Theorem exprD_mentionsU_strength_multi : forall tu e,
-    (forall n, length tu <= n -> mentionsU n e = false) ->
-    forall tg t tu',
-      exprD (Expr := @Expr_expr ts _ _) (tu ++ tu') tg e t =
-      exprD (Expr := @Expr_expr ts _ _) tu tg e t.
-  Proof.
-    intros; unfold exprD.
-    rewrite split_env_app.
-    destruct (split_env tg); destruct (split_env tu').
-    consider (split_env tu); intros.
-    simpl.
-    cutrewrite (length tu = length x1) in H.
-    { generalize (exprD'_mentionsU_strengthen_multi _ e H x t x0).
-      intros;
-        repeat match goal with
-                 | _ : match ?X with _ => _ end |- _ =>
-                   destruct X; intuition
-               end.
-      f_equal. eapply H1. }
-    { rewrite split_env_length. rewrite H0. reflexivity. }
-  Qed.
-
-End mentionsU.
-*)
-
-(*
-Section getInstantiation.
-  Require Import MirrorCore.ExprI.
-
-  
-  Variable func : Type.
-  Variable Subst_T : Subst T (expr func).
-
-  Definition getInstantiation (s : T) : uvar -> nat -> option (list (expr func)) :=
-    (fix recurse f l : option (list (expr func)) :=
-       match l with
-         | 0 => Some nil
-         | S n =>
-           match lookup f s with
-             | None => None
-             | Some z =>
-               match recurse (S f) n with
-                 | None => None
-                 | Some zs' => Some (z :: zs')
-               end
-           end
-       end).
-
-  Variable ts : types.
-  Variable RSym_func : RSym (typD ts) func.
-  Variable SubstOk : SubstOk (Expr_expr _) Subst_T.
-  Variable NormalizedSubstOk : NormalizedSubstOk Subst_T (@mentionsU func).
-
-  Lemma getInstantiation_S : forall s b a,
-    getInstantiation s a (S b) =
-    match lookup a s with
-      | None => None
-      | Some e => match getInstantiation s (S a) b with
-                    | None => None
-                    | Some es => Some (e :: es)
-                  end
-    end.
-  Proof. reflexivity. Qed.
-
-  Lemma getInstantiation_0 : forall s a,
-    getInstantiation s a 0 = Some nil.
-  Proof. reflexivity. Qed.
-
-  Lemma getInstantiation_contains_each : forall s b a i,
-    getInstantiation s a b = Some i ->
-    forall n,
-      n < b ->
-      exists e,
-        lookup (a + n) s = Some e /\
-        nth_error i n = Some e.
-  Proof.
-    induction b; intros.
-    { exfalso. omega. }
-    { rewrite getInstantiation_S in *.
-      consider (lookup a s); try congruence; intros.
-      consider (getInstantiation s (S a) b); try congruence; intros.
-      inv_all; subst.
-      specialize (IHb _ _ H1).
-      destruct n.
-      { rewrite Plus.plus_0_r. rewrite H. simpl; eauto. }
-      { rewrite <- plus_n_Sm. eapply IHb. omega. } }
-  Qed.
-
-  Lemma nth_error_Some_len : forall T (ls : list T) n v,
-    nth_error ls n = Some v ->
-    n < length ls.
-  Proof.
-    induction ls; destruct n; simpl; unfold error, value; intros; try congruence.
-    omega. eapply IHls in H. omega.
-  Qed.
-
-  Lemma WellTyped_getInstantiation : forall s us vs us' i,
-    WellTyped_subst (SubstOk := SubstOk) (us ++ us') vs s ->
-    getInstantiation s (length us) (length us') = Some i ->
-    forall n,
-      match nth_error us' n with
-        | None => True
-        | Some t =>
-          exists e,
-               nth_error i n = Some e
-            /\ Safe_expr (Expr := Expr_expr _) us vs e t
-      end.
-  Proof.
-    intros.
-    specialize (getInstantiation_contains_each _ _ H0); intro.
-    consider (nth_error us' n); auto; intros.
-    generalize (nth_error_Some_len _ _ H2); intro.
-    destruct (H1 _ H3).
-    exists x.
-    intuition.
-    destruct (WellTyped_lookup _ _ _ _ H H5).
-    rewrite nth_error_app_R in H4. 2: omega.
-    cutrewrite (length us + n - length us = n) in H4; try omega.
-    rewrite H2 in *. intuition; inv_all; subst.
-    unfold Safe_expr in *; simpl in *.
-    admit. (*
-    rewrite typeof_expr_mentionsU_strengthen_multi in H8.
-    eapply H8.
-    intros.
-    consider (length (us ++ us') ?[ le ] n0).
-    { intros; eapply mentionsU_WellTyped with (n := n0); eauto. }
-    { intros.
-      destruct NormalizedSubstOk.
-      destruct (H1 (n0 - length us)).
-      { rewrite app_length in H7; omega. }
-      { eapply lookup_normalized; try eassumption.
-        replace (length us + (n0 - length us)) with n0 in H9 by omega.
-        intuition eauto. } } *)
-  Qed.
-End getInstantiation.
-*)
-
-(*
-Section substU.
-  Variable typ : Type.
-  Variable func : Type.
-  Variable u : uvar.
-  Variable e' : expr typ func.
-
-  (** This replaces [UVar under] with [e] doing the appropriate
-   ** lifing.
-   **)
-  Fixpoint substU (under : nat) (e : expr typ func) : expr typ func :=
-    match e with
-      | Var _ => e
-      | Inj _ => e
-      | App l r => App (substU under l) (substU under r)
-      | Abs t e => Abs t (substU (S under) e)
-      | UVar u' =>
-        if u ?[ eq ] u' then
-          lift 0 under e'
-        else UVar u'
-    end.
-End substU.
-*)
+End instantiate_thm.
